\documentclass[problem]{mcs}

\begin{pcomments}
  \pcomment{CP_2_layer_array_network}
  \pcomment{from: S09.final}
\end{pcomments}

\pkeywords{
  networks
  congestion
  routing
}

%%%%%%%%%%%%%%%%%%%%%%%%%%%%%%%%%%%%%%%%%%%%%%%%%%%%%%%%%%%%%%%%%%%%%
% Problem starts here
%%%%%%%%%%%%%%%%%%%%%%%%%%%%%%%%%%%%%%%%%%%%%%%%%%%%%%%%%%%%%%%%%%%%%

\begin{problem}


Prove by induction that the $n^{th}$ perfect square is equal to the sum of the first $n$ odd numbers. That is, $\displaystyle{\sum_{i=1}^n(2n + 1) = (n+1)^2}$.


 \begin{solution}
Let $P(n)::= \displaystyle{\sum_{i=1}^n(2n + 1) = (n+1)^2}$.

We prove by induction that $P(n)$ is true for all $n$.

Base case: for $n = 0$, we have $1 = 1$, which is true, proving the base case.

Inductive step: assume that $P(n) \Rightarrow P(n+1)$.

We assume $P(n)$. So, $\displaystyle{\sum_{i=1}^n(2n + 1) = (n+1)^2}$. Now, we add $2(n+1) + 1$ to both sides of the equation.

It follows that $\displaystyle{\sum_{i=1}^{n+1}(2n + 1) = n^2 + 4n + 4 = ((n+1) + 1)^2}$ which proves $P(n+1)$. So, by induction, $P(n)$ is true for all $n$.
 \end{solution}


\end{problem}

\endinput
