\pcomment{CP_dependent_intransitive}

$A,B,C$ independent, $p \eqdef \pr{A} =  \pr{B}$, $r \eqdef \pr{C}$.

\[\pr{A \QXOR B} = 2p(1-p)\]

\[\pr{A \QXOR C} = p(1-r) + (1-p)r = p + r -2pr = \pr{B \QXOR C}\]

\[(A \QXOR B) \QAND (A \QXOR C) = A\bar{B}\bar{C} \QOR \bar{A}BC\]

\[\pr{(A \QXOR B) \QAND (A \QXOR C)} = p(1-p)(1-r) + (1-p)pr = p(1-p)[(1-r) + r] = p(1-p)\]

\[
\pr{A \QXOR B}\pr{A \QXOR C}
   = 2p(1-p)(p+r-2pr)
   = 2(p-p^2)(p+r-2pr)
   = 2(p^2+pr-2p^2r - p^3 - p^2r + 2p^3r)
   = 2(p^2 + pr -3p^2r -p^3 +2p^3r)
\]

\[2(p^2 + pr -3p^2r -p^3 +2p^3r) = p-p^2\]

\[-p + 3p^2 +2pr -6p^2r - 2p^3 + 4p^3r = 0\]

(define (T p r)
  (+ (- p)
     (* 3 p p )
     (* 2 p r)
     (* (- 6) p p r)
     (* (- 2) p p p)
     (* 4 p p p r)))

\[(A \QXOR C) \QAND (B \QXOR C) = \bar{A}\bar{B}C + AB\bar{C}\]

\[\pr{(A \QXOR C) \QAND (B \QXOR C)} = (1-p)^2 r+ p^2(1-r)\]

\[(1-p)^2 r+ p^2(1-r)+[2(p+r-2pr)(p^2-p)\]

r-2pr+p^2 +p^2 - p^2r + 2p^3 - 2p^2 + 2p^2 r - 2pr - 4p^3 r + 4p^2 r
   = r - 4pr - p^2 + 5p^2 r + 2p^3 - 4p^3 r

(define (Q p r)
  (+ r
     (* (- 4) p r)
     (* (- p) p)
     (* 5 p p r)
     (* 2 p p p)
     (* (- 4) p p p r)))


r - 4/3 r -1/9 +5/9 r + 2/27 - 4/27 r  (p = 1/3)

- 1/3 r -1/27 + 11/27 r

2/27 r = 1/27

(r = 1/2)


r - 4pr - p^2 + 5p^2 r + 2p^3 - 4p^3 r   (p = 2/3)

r - 8/3 r - 4/9 + 20/9 r + 16/27 - 32/27 r

-45/27 r  + 4/27 + 60/27 r - 32/27 r

-17/27 r = - 4/27

(r = 4/17)
