\documentclass[problem]{mcs}

\begin{pcomments}
  \pcomment{CP_sum_dif_frac}
\end{pcomments}

\pkeywords{
  sums
  summation
  telescoping
}

%%%%%%%%%%%%%%%%%%%%%%%%%%%%%%%%%%%%%%%%%%%%%%%%%%%%%%%%%%%%%%%%%%%%%
% Problem starts here
%%%%%%%%%%%%%%%%%%%%%%%%%%%%%%%%%%%%%%%%%%%%%%%%%%%%%%%%%%%%%%%%%%%%%

\begin{problem}
Find a closed-form for the following sums:
\bparts

\ppart 
\[
\sum_{i=1}^{n} \paren{\frac{1}{i+2012} - \frac{1}{i+2013}}\, .
\]

\begin{solution}
\begin{align*}
\lefteqn{sum_{i=1}^{n} \paren{\frac{1}{i+2012} - \frac{1}{i+2013}}}\\
 & = \paren{\frac{1}{2013} - \frac{1}{2014}} + \paren{frac{1}{2014} - frac{1}{2015}} +\\
 & \qquad  \cdots + \paren{\frac{1}{n+2012}- \frac{1}{n+2013}}\\
 & = \frac{1}{2013} + \paren{- \frac{1}{2014} + frac{1}{2014}} + \paren{-frac{1}{2015} + frac{1}{2015}} +\\
 & \qquad \cdots + \paren{-\frac{1}{n+2012} + \frac{1}{n+2012}} - \frac{1}{n+2013}\\
 & = \frac{1}{2013} - \frac{1}{n+2013}.
\end{align*}
\end{solution}

\ppart 
\[
\sum_{i=1}^{n} i^3\, .
\]

\begin{solution}
As noted in 13.2, the sum of the consecutive cubes might result in a fourth-degree polynomial in $n$.

$$\sum_{i=1}^{n} i^3 = an^4 + bn^3 + cn^2 + dn + e$$

We need to determine the coefficients.

$n=0$ implies $0 = e$

$n=1$ implies $1 = a + b + c + d + e$

$n=2$ implies $9 = 16a + 8b + 4c + 2d + e$

$n=3$ implies $36 = 81a + 27b + 9c + 3d+ e$

$n=4$ implies $100 = 256a + 64b + 16c + 4d + e$

Solving this equation gives: $a = \frac{1}{4}$, $b = \frac{1}{2}$, $c = \frac{1}{4}$, $d = 0$, $e = 0$.

Thus, 

$$ \sum_{i=1}^{n} i^3 = \frac{1}{4} (n^2 + n)^2 $$

This formula can be easily proved by induction.
\end{solution}

\eparts

\end{problem}

%%%%%%%%%%%%%%%%%%%%%%%%%%%%%%%%%%%%%%%%%%%%%%%%%%%%%%%%%%%%%%%%%%%%%
% Problem ends here
%%%%%%%%%%%%%%%%%%%%%%%%%%%%%%%%%%%%%%%%%%%%%%%%%%%%%%%%%%%%%%%%%%%%%

\endinput
