\documentclass[problem]{mcs}

\begin{pcomments}
  \pcomment{from: S09.cp11r}
  \pcomment{edited in-class probelm binom-coef to include in MQ}
\end{pcomments}

\pkeywords{
  binomial
  coefficients
}

%%%%%%%%%%%%%%%%%%%%%%%%%%%%%%%%%%%%%%%%%%%%%%%%%%%%%%%%%%%%%%%%%%%%%
% Problem starts here
%%%%%%%%%%%%%%%%%%%%%%%%%%%%%%%%%%%%%%%%%%%%%%%%%%%%%%%%%%%%%%%%%%%%%

\begin{problem}


\bparts

\ppart Define the sequence $r_0, r_1, r_2, \dots$ recursively by the
rule that $r_0=r_1=0$ and
\[
     r_n = 7r_{n-1}  +  4r_{n-2}  + (n+1),
\]           for $n\geq 2 $.  Express the generating function of this
sequence as a
quotient of polynomials or products of polynomials.  You do \emph{not}
have to find a closed form for $r_n$.

\begin{solution}
  Reasoning as in the derivation of the generating
  function for the orginal Fibonacci numbers, we have
\[
\begin{array}{rcrcrcrcrcr}
R(x)      & = & r_0 & + & r_1  x & + & r_2 x^2 & + & r_3 x^3 & + & r_4 x^4 + \cdots.\\
-7xR(x)   & = &     & - & 7r_0  x & - & 7r_1 x^2 & - & 7r_2 x^3 & - & 7r_3 x^4 - \cdots.\\
-4x^2R(x) & = &     &   &        & - & 4r_0 x^2 & - & 4r_1 x^3 & - & 4r_2 x^4 - \cdots.\\
\hline
R(x)(1-7x-4x^2) 
         & = & r_0 & + & (r_1-7r_0) 
                              x & + & (r_2 - 7r_1 - 4r_0)
                                          x^2 & + & \cdots & & \\
         & = &  0  & + & 0     & + & 3 x^2 & + & 4 x^3 + \cdots.\\
\end{array}
\]

Let the right hand side be $F(x)$, we have $F(x)=3x^2 + 4x^3 + 5x^4 +
\cdots$. 
\[
 F(x) - xF(x) = 3x^2 + x^3 + x^4 + \cdots = G(x)
\]
 \[ 
  G(x) - xG(x) = 3x^2 - 2x^3  \Longrightarrow G(x) = \frac{3x^2 -
    2x^3}{1-x} 
 \]
 We have $F(x) = \frac{G(x)}{1-x} = \frac{3x^2 - 2x^3}{(1-x)^2}$, 

so
\begin{equation}\label{Rfracx1}
R(x) = \frac{F(x)}{1 - 7x - 4x^2} = \frac{2x^2 - 2x^3}{(1-x)^2(1-7x-4x^2)}\, .
\end{equation}

\end{solution}




\iffalse
\ppart
 $x^8$ in $(x+x^3)^{4}$
\begin{solution}
$(x+x^3)^{4}$ can be expressed as $x^4(1+x^2)^4$.
\[
\binom{4}{2} = 6
\]
\end{solution}
\fi

\ppart Find the coefficients of $x^4y^{12}$ in $(7x+14y)^{16}$

\begin{solution}
\[
\binom{16}{4}7^414^{12}.
\]

When $(7x+14y)^{16}$ is expressed as a sum of powers of the summands
$7x$
and $14y$, the coefficient of $(7x)^4(14y)^{12}$ is $\binom{16}{4}$,
so the
coefficient of $x^4y^{12}$ is this binomial coefficient times
$7^4\cdot 14^{12}$.
\end{solution}

\eparts
\end{problem}


%%%%%%%%%%%%%%%%%%%%%%%%%%%%%%%%%%%%%%%%%%%%%%%%%%%%%%%%%%%%%%%%%%%%%
% Problem ends here
%%%%%%%%%%%%%%%%%%%%%%%%%%%%%%%%%%%%%%%%%%%%%%%%%%%%%%%%%%%%%%%%%%%%%
\endinput