\documentclass[problem]{mcs}

\begin{pcomments}
  \pcomment{MQ_wop_proof_sumofevens}
  \pcomment{new problem S14}
\end{pcomments}

\pkeywords{
  wop proof
}

%%%%%%%%%%%%%%%%%%%%%%%%%%%%%%%%%%%%%%%%%%%%%%%%%%%%%%%%%%%%%%%%%%%%%
% Problem starts here
%%%%%%%%%%%%%%%%%%%%%%%%%%%%%%%%%%%%%%%%%%%%%%%%%%%%%%%%%%%%%%%%%%%%%

\begin{problem}
Prove, using the Well Ordering Principle (WOP), that the sum of the smallest
$n$ {\em even, positive} integers is equal to $n(n+1)$.
\begin{solution}
We want to prove the following identity:
\[
\sum_{i=1}^n 2i = n(n+1)  
\]
for all non-negative integers $n$. The proof is by contradiction. Suppose to the contrary that the equation failed for some $n
\geq 0$.  Then by the WOP, there is a smallest nonnegative integer,
$m$, such this formula does not hold when $n = m$.

But the formula clearly holds when $n = 1$, which means that $m \geq
2$.  Therefore $m-1$ is positive and since it is smaller than $m$,
the formula must be true for $n = m-1$.  That is,
\begin{equation}\label{sum-to-m-1}
\sum_{i=0}^{m-1} 2i = (m-1)m.
\end{equation}
Let us add $2m$ to both sides of equation~\eqref{sum-to-m-1}.
Then, the left hand side equals
\[
2m + \sum_{i=0}^{m-1} 2i \; ,
\]
while the right hand side equals
\[
2m + (m-1)m = 2m + m^2 - m \; .
\]
Simplifying, we get
\[
\sum_{i=0}^{m} 2m = m+m^2 = m(m+1) \; ,
\]
contradicting the fact that our formula does not hold for
$m$.

\end{solution}

\end{problem}


%%%%%%%%%%%%%%%%%%%%%%%%%%%%%%%%%%%%%%%%%%%%%%%%%%%%%%%%%%%%%%%%%%%%%
% Problem ends here
%%%%%%%%%%%%%%%%%%%%%%%%%%%%%%%%%%%%%%%%%%%%%%%%%%%%%%%%%%%%%%%%%%%%%
\endinput
