\documentclass[problem]{mcs}

\begin{pcomments}
  \pcomment{MQ_wop_prooof_sumofodds}
  \pcomment{by ARM 8/22/11}
\end{pcomments}

\pkeywords{
  well ordering
  sum
}

%%%%%%%%%%%%%%%%%%%%%%%%%%%%%%%%%%%%%%%%%%%%%%%%%%%%%%%%%%%%%%%%%%%%%
% Problem starts here
%%%%%%%%%%%%%%%%%%%%%%%%%%%%%%%%%%%%%%%%%%%%%%%%%%%%%%%%%%%%%%%%%%%%%

\begin{problem}

Prove \emph{by the Well Ordering Principle}\footnote{Proofs by other
  methods such as induction will not receive full credit.} that the
sum of the first $n$ odd numbers is $n^2$, that is,
\begin{equation}\label{sumofodds}
\sum_{i=1}^{n} (2(i-1)+1) = n^2.
\end{equation}

\begin{solution}
The proof is by contradiction.

Suppose to the contrary that equation~\eqref{sumofodds} failed for
some $n \geq 1$.  Then by the WOP, there is a \emph{smallest} integer,
$m \geq 1$, such this formula does not hold when $n = m$.

But when $n=1$, both sides of~\eqref{sumofodds} equal 1, so it must be
that $m \geq 2$.  In particular, $m-1 \geq 1$.  Since $m-1 < m$, and
$m$ is the smallest number $\geq 1$ for which
equation~\eqref{sumofodds} fails, the equation must be true for $n =
m-1$.  That is,
\begin{equation}\label{sumodds-to-m-1}
\sum_{i=1}^{m-1} (2(i-1)+1) = (m-1)^2.
\end{equation}
Now add $2(m-1)+1$ to both sides of equation~\eqref{sumodds-to-m-1}.
Then the left hand side equals
\[
\paren{\sum_{i=1}^{m-1} (2(i-1)+1)} + (2(m-1)+1) = \sum_{i=1}^{m} (2(i-1)+1),
\]
and the right hand side equals
\[
(m-1)^2 + (2(m-1)+1) = (m^2 -2m + 1) + (2m - 2 + 1) = m^2.
\]
That is,
\[
\sum_{i=1}^{m} (2(i-1)+1) = m^2,
\]
contradicting the fact that equation~\eqref{sumodds-to-m-1} does not hold for
$m$.

\end{solution}

\end{problem}


%%%%%%%%%%%%%%%%%%%%%%%%%%%%%%%%%%%%%%%%%%%%%%%%%%%%%%%%%%%%%%%%%%%%%
% Problem ends here
%%%%%%%%%%%%%%%%%%%%%%%%%%%%%%%%%%%%%%%%%%%%%%%%%%%%%%%%%%%%%%%%%%%%%
\endinput
